tmp

theories/ELF.v
@@ -1,4 +1,5 @@
-Require Import Util PString Lia Strl Rewrite.
+From coqutil Require Import bitblast.
+Require Import Util PString Lia Strl Rewrite ZArith.
 From RecordUpdate Require Import RecordUpdate.
 
 Notation getu8 := slget.
@@ -11,6 +12,21 @@ Definition u8 i := i land 0xff::nil.
 Definition u16 i :=  u8 i ++  u8 (i >> 8).
 Definition u32 i := u16 i ++ u16 (i >> 16).
 Definition u64 i := u32 i ++ u32 (i >> 32).
+
+Definition u8_equiv : forall {s s' i} (E: s ≡ s'), getu8 s i = getu8 s' i := equiv_get.
+Definition u16_equiv : forall {s s' i} (E: s ≡ s'), getu16 s i = getu16 s' i.
+Proof. intros. unfold getu16. now rewrite !(u8_equiv E). Qed.
+Definition u32_equiv : forall {s s' i} (E: s ≡ s'), getu32 s i = getu32 s' i.
+Proof. intros. unfold getu32. now rewrite !(u16_equiv E). Qed.
+Definition u64_equiv : forall {s s' i} (E: s ≡ s'), getu64 s i = getu64 s' i.
+Proof. intros. unfold getu64. now rewrite (u8_equiv E), !(u32_equiv E). Qed.
+Definition u8_before : forall s i j (J: i <? j = true), getu8 s i = getu8 (slsub s 0 j) i := get_before.
+Definition u16_before : forall s i j (I: (to_Z i < wB - 1)%Z) (J: i + 1 <? j = true), getu16 s i = getu16 (slsub s 0 j) i.
+Proof. intros. unfold getu16. now rewrite (u8_before s i j), (u8_before s (i+1) j) by lia. Qed.
+Definition u32_before : forall s i j (I: (to_Z i < wB - 3)%Z) (J: i + 3 <? j = true), getu32 s i = getu32 (slsub s 0 j) i.
+Proof. intros. unfold getu32. now rewrite (u16_before s i j), (u16_before s (i+2) j) by lia. Qed.
+Definition u64_before : forall s i j (I: (to_Z i < wB - 7)%Z) (J: i + 7 <? j = true), getu64 s i = getu64 (slsub s 0 j) i.
+Proof. intros. unfold getu64. now rewrite (u32_before s i j), (u32_before s (i+4) j), (u8_before s (i+7) j) by lia. Qed.
 
 Definition ELFMAG := 0x464c457f.
 Definition ELFCLASS64 := 2.
@@ -60,13 +76,13 @@ Record ELF := {
   data: list string;
 }.
 
-Definition parse_eident s :=
-  let ei_mag := getu32 s 0 in
-  let ei_class := getu8 s 4 in
-  let ei_data := getu8 s 5 in
-  let ei_version := getu8 s 6 in
-  let ei_osabi := getu8 s 7 in
-  let ei_abiversion := getu8 s 8 in
+Definition parse_eident bin :=
+  let ei_mag := getu32 bin 0 in
+  let ei_class := getu8 bin 4 in
+  let ei_data := getu8 bin 5 in
+  let ei_version := getu8 bin 6 in
+  let ei_osabi := getu8 bin 7 in
+  let ei_abiversion := getu8 bin 8 in
   assert ei_mag =? ELFMAG;
   assert ei_class =? ELFCLASS64;
   assert ei_version =? EV_CURRENT;
@@ -78,22 +94,24 @@ Definition parse_eident s :=
     ei_osabi := ei_osabi;
     ei_abiversion := ei_abiversion;
   |}.
-Definition parse_ehdr s :=
-  e_ident ← parse_eident s;
-  let e_type := getu16 s 16 in
-  let e_machine := getu16 s 18 in
-  let e_version := getu32 s 20 in
-  e_entry ← getu64 s 24;
-  e_phoff ← getu64 s 32;
-  e_shoff ← getu64 s 40;
-  let e_flags := getu32 s 48 in
-  let e_ehsize := getu16 s 52 in
-  let e_phentsize := getu16 s 54 in
+Definition parse_ehdr bin :=
+  e_ident ← parse_eident bin;
+  let e_type := getu16 bin 16 in
+  let e_machine := getu16 bin 18 in
+  let e_version := getu32 bin 20 in
+  e_entry ← getu64 bin 24;
+  e_phoff ← getu64 bin 32;
+  assert 64 <? e_phoff;
+  e_shoff ← getu64 bin 40;
+  let e_flags := getu32 bin 48 in
+  let e_ehsize := getu16 bin 52 in
+  let e_phentsize := getu16 bin 54 in
   assert e_phentsize =? 56;
-  let e_phnum := getu16 s 56 in
-  let e_shentsize := getu16 s 58 in
-  let e_shnum := getu16 s 60 in
-  let e_shstrndx := getu16 s 62 in
+  let e_phnum := getu16 bin 56 in
+  assert e_phoff <? e_phoff + 56 * e_phnum;
+  let e_shentsize := getu16 bin 58 in
+  let e_shnum := getu16 bin 60 in
+  let e_shstrndx := getu16 bin 62 in
   return {|
     e_ident := e_ident;
     e_type := e_type;
@@ -110,15 +128,15 @@ Definition parse_ehdr s :=
     e_shnum := e_shnum;
     e_shstrndx := e_shstrndx;
   |}.
-Definition parse_phdr_at s i :=
-  let p_type := getu32 s i in
-  let p_flags := getu32 s (i+4) in
-  p_offset ← getu64 s (i+8);
-  p_vaddr ← getu64 s (i+16);
-  p_paddr ← getu64 s (i+24);
-  p_filesz ← getu64 s (i+32);
-  p_memsz ← getu64 s (i+40);
-  p_align ← getu64 s (i+48);
+Definition parse_phdr_at bin i :=
+  let p_type := getu32 bin i in
+  let p_flags := getu32 bin (i+4) in
+  p_offset ← getu64 bin (i+8);
+  p_vaddr ← getu64 bin (i+16);
+  p_paddr ← getu64 bin (i+24);
+  p_filesz ← getu64 bin (i+32);
+  p_memsz ← getu64 bin (i+40);
+  p_align ← getu64 bin (i+48);
   return {|
     p_type := p_type;
     p_flags := p_flags;
@@ -132,21 +150,36 @@ Definition parse_phdr_at s i :=
 Function range step i n {measure to_nat n} :=
   if (n =? 0) then nil else i::range step (i+step) (n-1).
 Proof. lia. Defined.
+Lemma range_len:
+  forall step i n, List.length (range step i n) = to_nat n.
+Proof.
+  intros. apply range_ind; intros. simpl. lia. simpl. rewrite H. lia.
+Qed.
 Definition phdr_offsets := range 56.
 Definition to_words sl := map (getu32 sl) (range 4 0 (sllength sl >> 2)).
 Definition of_chunks32 (lli: list (list int)) := map (λ x, of_list (List.concat (map_single u32 x))) lli.
 Definition of_chunks64 (lli: list (list int)) := flat_map (λ x, (map (λ y, of_list (u64 y)) x)) lli.
-Definition parse_phdr s ehdr :=
+Definition parse_phdr bin ehdr :=
   let n := ehdr.(e_phnum) in
   assert negb (n =? 0xffff);
-  maybe_map (parse_phdr_at s) (phdr_offsets ehdr.(e_phoff) n).
+  maybe_map (parse_phdr_at bin) (phdr_offsets ehdr.(e_phoff) n).
 Definition parse_elf data :=
+  assert 64 <? sllength data;
   ehdr ← parse_ehdr data;
   phdrs ← parse_phdr data ehdr;
   return {| ehdr := ehdr; phdrs := phdrs; data := data |}.
 
 Fixpoint findn {A} (f:A -> bool) l n :=
   match l with | nil => None | a::t => if (f a) then Some n else findn f t (n+1) end.
+Lemma findn_bound:
+  forall A f l n m, findn f l m = Some n -> to_nat n < to_nat m + @List.length A l.
+Proof.
+  induction l; simpl; intros.
+    easy.
+    destruct f.
+      injection H. lia.
+      apply IHl in H. lia.
+Qed.
 Definition is_txt_seg p := (p.(p_type) =? PT_LOAD) && (bit p.(p_flags) 0).
 
 Definition replaceable_seg phdrs :=
@@ -154,6 +187,13 @@ Definition replaceable_seg phdrs :=
   | None => (findn (λ x, x.(p_type) =? PT_NOTE) phdrs 0)
   | Some n => Some n
   end.
+Lemma replaceable_seg_bound:
+  forall phdrs n, replaceable_seg phdrs = Some n -> to_nat n < List.length phdrs.
+Proof.
+  intros. unfold replaceable_seg in H. destruct findn eqn:E.
+    apply findn_bound in E. injection H. lia.
+    now apply findn_bound in H.
+Qed.
 Definition txt_seg elf := find is_txt_seg elf.(phdrs).
 Definition load_seg offset vaddr content :=
   Build_Phdr PT_LOAD PF_RX offset vaddr vaddr (sllength content) (sllength content) 0x1000.
@@ -168,7 +208,19 @@ Definition phdr_data p :=
     u64 p.(p_memsz)::
     u64 p.(p_align)::nil
   ).
-
+Lemma landland:
+  forall a b, a land b land b = a land b.
+Proof. zify. apply Z.bits_inj. intro. rewrite !Z.land_spec. lia. Qed.
+Lemma phdr_data_len:
+  forall p, List.length (LO (phdr_data p)) = 56%nat.
+Proof.
+  intros. unfold list_of_strl, phdr_data. 
+  cbv [map]. rewrite !to_of_list.
+  all: easy || unfold u64, u32, u16, u8, char63_valid; repeat constructor.
+  all: now rewrite landland.
+Qed.
+Lemma addl: forall i j, i <? i + j = true -> (to_Z i + to_Z j < wB)%Z.
+Proof. lia. Qed.
 Definition listreplace {A} l n (x:A) := firstn n l++x::skipn (S n) l.
 Definition replace_phdr elf phdr i :=
   let phdr_offset := elf.(ehdr).(e_phoff) + 56 * i in
@@ -179,6 +231,7 @@ Definition map_phdrs (f: Phdr -> option Phdr) elf :=
   fst (fold_left g elf.(phdrs) (elf, 0)).
 Definition with_load_seg elf content vaddr :=
   idx ← replaceable_seg elf.(phdrs);
+  assert elf.(ehdr).(e_phoff) + 56 * idx <? sllength elf.(data);
   let padding := (0x1000 - sllength elf.(data) land 0xfff) land 0xfff in
   let offset := sllength elf.(data) + padding in
   let elf := replace_phdr elf (load_seg offset vaddr content) idx in
@@ -234,6 +287,7 @@ Lemma parse_elf_data:
 Proof.
   intros. repeat so E. now subst.
 Qed.
+Lemma add_0_int: forall i, i = 0 + i. Proof. lia. Qed.
 Lemma eident_same {bin eident bin'}
   (E: parse_eident bin = Some eident)
   (S: slsub bin 0 64 ≡ slsub bin' 0 64):
@@ -246,10 +300,10 @@ Proof.
            | |- context [getu8 _ ?A] =>
                lazymatch A with
                | 0 + _ => fail
-               | _ => replace A with (0 + A) by lia
+               | _ => rewrite (add_0_int A)
                end
            end;
-    rewrite !(sub_equiv bin' bin 0 64); auto; lia.
+    rewrite !(sub_equiv_get bin' bin 0 64); auto; lia.
 Qed.
 Lemma ehdr_same {bin ehdr bin'}
   (E: parse_ehdr bin = Some ehdr)
@@ -263,32 +317,246 @@ Proof.
            | |- context [getu8 _ ?A] =>
                lazymatch A with
                | 0 + _ => fail
-               | _ => replace A with (0 + A) by lia
+               | _ => rewrite (add_0_int A)
                end
            end;
-    rewrite !(sub_equiv bin' bin 0 64); auto; lia.
+    try (rewrite !(sub_equiv_get bin' bin 0 64); auto); lia.
+Qed.
+Lemma maybe_map_len:
+  forall A B (f: A -> option B) l l', maybe_map f l = Some l' -> List.length l' = List.length l.
+Proof.
+  intros. unfold maybe_map, mapfold in H.
+  generalize l l' H. clear. induction l; intros. now inversion H.
+  repeat so H. apply IHl in H1. subst. simpl. lia.
 Qed.
 
+Lemma phdr_len:
+  forall s ehdr p, parse_phdr s ehdr = Some p -> List.length p = to_nat ehdr.(e_phnum).
+Proof.
+  intros. do 2 so H. apply maybe_map_len in H. unfold phdr_offsets in H. now rewrite range_len in H.
+Qed.
+Variant IsPhoff (data: list string) : int -> Prop :=
+  | isphoff i (I: getu64 data 32 = Some i) : IsPhoff data i.
+Variant IsPhnum (data: list string) : int -> Prop :=
+  | isphnum i (I: getu16 data 56 = i) : IsPhnum data i.
+Variant IsPhdr (data: list string) : list string -> Prop :=
+  | isphdr phoff phnum i p
+      (O: IsPhoff data phoff)
+      (N: IsPhnum data phnum)
+      (I: i <? phnum = true)
+      (P: slsub data (phoff + 56 * i) 56 ≡ p) : IsPhdr data p.
+Variant IsLoad (seg: list string) : Prop :=
+  | isload (S: getu32 seg 0 = PT_LOAD).
+Variant IsRX (seg: list string) : Prop :=
+  | isrx (S: getu32 seg 4 = PF_RX).
+Variant HasOffset (seg: list string) : int -> Prop :=
+  | hasoffset offset (S: getu64 seg 8 = Some offset) : HasOffset seg offset.
+Variant IsAt (seg: list string) : int -> Prop :=
+  | isat vaddr (S: getu64 seg 16 = Some vaddr) : IsAt seg vaddr.
+Variant HasSize (seg: list string) : int -> Prop :=
+  | haslength filesz (S: getu64 seg 32 = Some filesz) : HasSize seg filesz.
+Variant HasContent (data: list string) (seg: list string) : list string -> Prop :=
+  | hascontent content offset vaddr filesz
+      (S: IsPhdr data seg)
+      (O: HasOffset seg offset)
+      (V: IsAt seg vaddr)
+      (F: HasSize seg filesz)
+      (C: slsub data offset filesz ≡ content) : HasContent data seg content.
+Lemma getu8_bound:
+  forall sl i, getu8 sl i <? 256 = true.
+Proof.
+  induction sl. easy. intros. simpl. destruct (ltb i). pose proof (get_char63_valid a i).
+  unfold char63_valid in H. zify. change 255%Z with (Z.ones 8) in H. rewrite Z.land_ones in H. lia. lia.
+  easy.
+Qed.
+Lemma getu16_bound:
+  forall sl i, getu16 sl i <? 0x10000 = true.
+Proof.
+  unfold getu16. intros. pose (getu8_bound sl i). pose (getu8_bound sl (i+1)). lia.
+Qed.
+Require I2N.
+Import I2N.notations.
+Require Import FunctionalExtensionality.
+Lemma getu64_sub:
+  forall sl i, (to_Z i + 8 <= wB)%Z -> getu64 sl i = getu64 (slsub sl i 8) 0.
+Proof.
+  intros. unfold getu64, getu32, getu16.
+  rewrite <-!add_assoc. simpl.
+  repeat match goal with |- context [getu8 sl (i + ?k)] => rewrite (get_sub sl (i + k) 8 (i)) end.
+  rewrite (get_sub sl i 8 i).
+  all: try lia.
+  remember (negb _). remember (negb _) in |-*. replace b0 with b. destruct b. simpl. 
+  repeat f_equal; lia. easy. subst. repeat f_equal. lia.
+Qed.
+Lemma getu64_equiv:
+  forall sl sl2 i, sl ≡ sl2 -> getu64 sl i = getu64 sl2 i.
+Proof.
+  intros. unfold getu64, getu32, getu16. now rewrite !(equiv_get _ _ _ H).
+Qed.
+Lemma makeu8:
+  forall a, of_list (u8 a) = make 1 a.
+Proof.
+  intros. simpl. apply to_list_inj. now rewrite cat_spec, !make_spec, landland.
+Qed.
+Lemma getu8_u8:
+  forall a, getu8 [of_list (u8 a)] 0 = a land 255.
+Proof.
+  intros. cbv.
+  now rewrite get_spec, length_spec_int, !cat_spec, make_spec, landland. 
+Qed.
+(* Infix ">>" := N.shiftr. *)
+(* Infix "<<" := N.shiftl. *)
+(* Infix ".&" := N.land (at level 30). *)
+From coqutil Require Import prove_Zeq_bitwise.
+(* Lemma getu16_u16: *)
+(*   forall a, getu16 [of_list (u16 a)] 0 = a land 0xffff. *)
+(* Proof. *)
+(*   intros. unfold getu16, u16. rewrite of_list_app, !makeu8. *)
+(*   rewrite !list_get. simpl. cbv[list_of_strl map concat]. *)
+(*   rewrite cat_spec_valid_length, !make_spec, app_nil_r by (rewrite !make_length_spec; lia). simpl. *)
+(*   I2N.zify. *)
+(*   unfold wB. *)
+(*   rewrite <-!Z.land_ones by lia. *)
+(*   rewrite <-!Z.or_to_plus. *)
+(*   prove_Zeq_bitwise. *)
+(*   prove_Zeq_bitwise. *)
+(* Qed. *)
+Lemma byte: forall i mask s, ((i >> s) land mask) << s = i land (mask << s).
+Proof.
+  intros. I2N.zify.
+  unfold wB. rewrite <-!Z.land_ones by lia.
+  prove_Zeq_bitwise. repeat f_equal. lia.
+Qed.
+Lemma lsl_add: forall a b s, (a + b) << s = a << s + b << s.
+Proof.
+  intros. I2N.zify. rewrite !Z.shiftl_mul_pow2 by lia. lia.
+Qed.
+Lemma lsr_lsr: forall a b c, (to_Z b + to_Z c < wB)%Z -> a >> b >> c = a >> (b + c).
+Proof.
+  intros. I2N.zify. unfold wB. rewrite Z.mod_small by lia.
+  prove_Zeq_bitwise.
+Qed.
+Lemma add_lor: forall a b, a land b = 0 -> a + b = a lor b.
+Proof.
+  intros. I2N.zify. apply eq_int_inj in H. rewrite I2N.I2Z.inj_land in H.
+  rewrite <-Z.or_to_plus by lia. unfold wB. rewrite <-Z.land_ones by lia.
+  rewrite Z.land_lor_distr_l. f_equal; rewrite Z.land_ones; lia.
+Qed.
+Lemma land2: forall a b c, (a land b) land (a land c) = a land (b land c).
+Proof. intros. now rewrite !landA, (landC a b), landland. Qed.
+Lemma lan: forall a b c d, (a land b) land (c land d) = (a land c) land (b land d).
+Proof. intros. I2N.zify. prove_Zeq_bitwise. Qed.
+Lemma getu64_u64: 
+  forall a, getu64 [of_list (u64 a)] 0 = Some a.
+Proof.
+  intros. unfold getu64, getu32, getu16, getu8.
+  remember (length _). simpl in Heqi.
+  rewrite length_spec_int in Heqi.
+  rewrite !cat_spec, !make_spec in Heqi. simpl in Heqi. cbv in Heqi.
+  subst i. cbv[ add ltb].
+  simpl.
+  rewrite !get_spec, !cat_spec, !nth_firstn, !make_spec.
+  repeat replace (_ <? _)%nat with true by lia.
+  repeat match goal with |- context[Nat.min ?a _] => replace (Nat.min a _) with a by lia end.
+  simpl. rewrite !landland. sog. sog. shelve.
+  rewrite land_spec, andb_true_r, !bit_lsr. simpl. rewrite bit_M by lia. lia. Unshelve.
+  rewrite !byte. rewrite !lsl_add, !byte.
+  rewrite !add_assoc. 
+  rewrite (add_lor (a land 255)) by now rewrite land2, land0_r.
+  rewrite (add_lor (_ lor _)). 
+  rewrite (add_lor (_ lor _)). 
+  rewrite (add_lor (_ lor _)). 
+  rewrite (add_lor (_ lor _)). 
+  rewrite (add_lor (_ lor _)). 
+  rewrite (add_lor (_ lor _)). 
+  I2N.zify. unfold wB. rewrite <-!Z.land_ones by lia. 
+  change (to_Z 0) with Z0. 
+ replace (to_Z a) with (Z.land (to_Z a) (Z.ones 63)) by (rewrite Z.land_ones; lia).
+  (* prove_Zeq_bitwise. *)
+  (* I2N.zify. unfold wB. rewrite <-!Z.land_ones by lia.  *)
+  (* change (to_Z 0) with Z0. prove_Zeq_bitwise. *)
+  (* I2N.zify. unfold wB. rewrite <-!Z.land_ones by lia.  *)
+  (* change (to_Z 0) with Z0. prove_Zeq_bitwise. *)
+  (* I2N.zify. unfold wB. rewrite <-!Z.land_ones by lia.  *)
+  (* change (to_Z 0) with Z0. prove_Zeq_bitwise. *)
+  (* I2N.zify. unfold wB. rewrite <-!Z.land_ones by lia.  *)
+  (* change (to_Z 0) with Z0. prove_Zeq_bitwise. *)
+  (* I2N.zify. unfold wB. rewrite <-!Z.land_ones by lia.  *)
+  (* change (to_Z 0) with Z0. prove_Zeq_bitwise. *)
+  (* I2N.zify. unfold wB. rewrite <-!Z.land_ones by lia.  *)
+  (* change (to_Z 0) with Z0. prove_Zeq_bitwise. *)
+Admitted.
 Theorem add_code_correct:
   forall bin bin' content addr
     (B: add_code bin content addr = Some bin'),
-  match parse_elf bin' with
-  | Some elf => Exists (λ s,
-      s.(p_type) = PT_LOAD
-      ∧ s.(p_flags) = PF_RX
-      ∧ s.(p_vaddr) = addr
-      ∧ slsub bin' s.(p_offset) s.(p_filesz) = content) elf.(phdrs)
-  | None => False
-  end.
+  exists seg,
+    IsPhdr bin' seg /\
+    IsLoad seg /\
+    IsRX seg /\
+    IsAt seg addr /\
+    HasContent bin' seg content.
 Proof.
-  intros.
-  repeat so B.
-  repeat so H0.
-  unfold parse_elf.
-  rewrite <-H0 in B. clear H0.
-  rewrite (parse_elf_data H) in B. simpl in B.
-  so H. so H.
-  epose proof (ehdr_same H0 _). rewrite H2. simpl.
+  intros. repeat so B. repeat so H0.
+  remember (phdr_data _). exists l.
+  repeat so H. repeat so H2.
+
+  assert (IsPhdr bin' l).
+  { subst x0 x. simpl in B.
+    apply replaceable_seg_bound in H1. simpl in H1. apply phdr_len in H3.
+    assert (slsub bin' 0 64 ≡ slsub bin 0 64).
+    { subst x2. simpl in *. 
+      pose proof (getu16_bound bin 56).
+      subst bin'. rewrite sub_cat1. erewrite splice_before. easy. easy. rewrite <-H. lia.
+      simpl. rewrite Zlength_correct, list_splice, length_app, length_firstn.
+      rewrite list_length in Heqb0. lia. }
+    econstructor.
+    + apply (isphoff _ x2.(e_phoff)).
+      erewrite (u64_before _ _ 64), u64_equiv, <-(u64_before _ _ 64), H6; lia || auto. now subst.
+    + apply (isphnum _ x2.(e_phnum)). 
+      erewrite (u16_before _ _ 64), u16_equiv, <-(u16_before _ _ 64); try lia. now subst. easy.
+    + assert (x1 <? e_phnum x2 = true). rewrite H3 in H1. lia. apply H0.
+    + rewrite B. rewrite sub_cat1, sub_splice. easy.
+      easy. subst l. rewrite Zlength_correct, phdr_data_len. easy.
+      rewrite Zlength_correct, list_splice, !length_app, length_firstn.
+      rewrite list_length in Heqb0. simpl in *. 
+      replace (Nat.min _ _) with (to_nat (e_phoff x2 + 56 * x1)) by lia.
+      subst l.
+      rewrite phdr_data_len. lia. }
+  assert (getu64 l 16 = Some addr).
+  { rewrite getu64_sub. rewrite (getu64_equiv _ (of_list (u64 addr)::nil)).
+    apply getu64_u64.
+    subst l.
+    rewrite list_sub. unfold list_of_strl, phdr_data.
+    cbv[map]. rewrite !to_of_list.
+  all: easy || unfold u64, u32, u16, u8, char63_valid; repeat constructor.
+  all: now rewrite landland.
+  }
+  repeat split.
+  - easy.
+  - subst. easy.
+  - subst. easy.
+  - easy. 
+  - eapply (hascontent _ _ _ _ addr (sllength content)). easy.
+    econstructor. rewrite getu64_sub by lia. erewrite (getu64_equiv _ (of_list (u64 _)::nil)).
+    apply getu64_u64. subst l.
+
+    rewrite list_sub. unfold list_of_strl, phdr_data.
+    cbv[map]. rewrite !to_of_list.
+  all: easy || unfold u64, u32, u16, u8, char63_valid; repeat constructor.
+  all: try now rewrite landland.
+     rewrite getu64_sub by lia. rewrite (getu64_equiv _ (of_list (u64 (sllength content))::nil)).
+    apply getu64_u64.
+    subst l.
+    rewrite list_sub. unfold list_of_strl, phdr_data.
+    cbv[map]. rewrite !to_of_list.
+  all: easy || unfold u64, u32, u16, u8, char63_valid; repeat constructor.
+  all: try now rewrite landland.
+    subst bin' x0. simpl.
+    erewrite equiv_sub; [|erewrite cat_splice; try reflexivity]. admit.
+    (* lia. *)
+    (* rewrite sub_cat2. *)
+    (* admit. rewrite Zlength_correct. rewrite list_splice, !length_app, length_firstn, length_skipn. *)
+    (* rewrite cat_splice. rewrite  *)
 Admitted.
 
 Definition rw_elf bin pol dsets abort :=
